src/kemedhoc/Impl.KEMEDHOC.CryptoPrimitives.fst
@@ -1,0 +1,62 @@
+module Impl.KEMEDHOC.CryptoPrimitives
+
+// open Lib.ByteBuffer
+// open Lib.Buffer
+// open Lib.ByteSequence
+// open Lib.IntTypes
+// open LowStar.BufferOps
+
+(*LowStar related modules*)
+module B = LowStar.Buffer
+module ST = FStar.HyperStack.ST
+module HS = FStar.HyperStack
+module S = FStar.Seq
+module Seq = Lib.Sequence
+
+(*Specification modules*)
+module Spec = Spec.KEMEDHOC.CryptoPrimitives
+
+// open Impl.KEMEDHOC.Types
+
+module ImplEdhocCrypto = Impl.EDHOC.CryptoPrimitives
+module SpecEdhocCrypto = Spec.EDHOC.CryptoPrimitives
+
+module ImplAEAD = EverCrypt.AEAD
+module SpecAEAD = Spec.Agile.AEAD
+
+/// Frodo Impl modules
+module ImplFrodo = Hacl.Frodo.KEM
+module ImplFrodoRand = Hacl.Frodo.Random
+
+module SpecHash = Spec.Agile.Hash
+module DefHash = Spec.Hash.Definitions
+
+// open Lib.RandomBuffer.System
+// open Lib.RandomSequence
+module HACLRandom = Lib.RandomSequence
+
+(*------------------ KEM*)
+
+/// KEM key generation
+let kem_keygen_frodo640 pk sk
+  = (**) let h0 = ST.get() in
+  ST.push_frame ();
+  let kem_entr_buf = create (size Spec.kem_entr_len) (u8 0) in
+  crypto_random kem_entr_buf (size Spec.kem_entr_len);
+  ImplFrodoRand.randombytes_init_ kem_entr_buf;
+  let _ = ImplFrodo.crypto_kem_keypair (Spec.kemAlg_to_frodo_alg Spec.Frodo640) Spec.genFrodoAlg pk sk in
+  ST.pop_frame ()
+
+/// KEM encapsulation
+let kem_encaps_frodo640 pk ct ss
+  = ST.push_frame ();
+  let kem_entr_buf = create (size Spec.kem_entr_len) (u8 0) in
+  crypto_random kem_entr_buf (size Spec.kem_entr_len);
+  ImplFrodoRand.randombytes_init_ kem_entr_buf;
+  let _ = ImplFrodo.crypto_kem_enc (Spec.kemAlg_to_frodo_alg Spec.Frodo640) Spec.genFrodoAlg ct ss pk in
+  ST.pop_frame ()
+
+/// KEM decapsulation
+let kem_decaps_frodo640 sk ct ss
+  = let _ = ImplFrodo.crypto_kem_dec (Spec.kemAlg_to_frodo_alg Spec.Frodo640) Spec.genFrodoAlg ss ct sk in
+  ()
