src/kemedhoc/Impl.KEMEDHOC.CryptoPrimitives.fsti
@@ -1,0 +1,171 @@
+module Impl.KEMEDHOC.CryptoPrimitives
+
+open Lib.ByteBuffer
+open Lib.Buffer
+open Lib.ByteSequence
+open Lib.IntTypes
+open LowStar.BufferOps
+
+(*LowStar related modules*)
+module B = LowStar.Buffer
+module ST = FStar.HyperStack.ST
+module HS = FStar.HyperStack
+module S = FStar.Seq
+module Seq = Lib.Sequence
+
+(*Specification modules*)
+module Spec = Spec.KEMEDHOC.CryptoPrimitives
+
+open Impl.KEMEDHOC.Types
+
+module ImplEdhocCrypto = Impl.EDHOC.CryptoPrimitives
+module SpecEdhocCrypto = Spec.EDHOC.CryptoPrimitives
+
+module ImplAEAD = EverCrypt.AEAD
+module SpecAEAD = Spec.Agile.AEAD
+
+/// Frodo Impl modules
+module ImplFrodo = Hacl.Frodo.KEM
+module ImplFrodoRand = Hacl.Frodo.Random
+
+module SpecHash = Spec.Agile.Hash
+module DefHash = Spec.Hash.Definitions
+
+open Lib.RandomBuffer.System
+// open Lib.RandomSequence
+module HACLRandom = Lib.RandomSequence
+
+/// Re-declare here the supportedKemCipherSuite type
+/// just for avoid typing the prefix `Spec`
+inline_for_extraction
+let supportedKemCipherSuite = Spec.supportedKemCipherSuite
+inline_for_extraction
+let supportedKemAlg = Spec.supportedKemAlg
+
+
+(*------------------ AEAD*)
+inline_for_extraction
+let aead_config_pre (kcs: supportedKemCipherSuite) = ImplAEAD.config_pre (Spec.get_aead_alg kcs)
+
+let aead_encrypt (kcs: supportedKemCipherSuite)
+  : ImplEdhocCrypto.aead_encrypt_st (Spec.get_aead_alg kcs) (aead_config_pre kcs)
+  = match (Spec.get_aead_alg kcs) with
+    | SpecAEAD.AES128_GCM -> ImplEdhocCrypto.aead_aes128_gcm_encrypt
+    | SpecAEAD.AES256_GCM -> ImplEdhocCrypto.aead_aes256_gcm_encrypt
+
+let aead_decrypt (kcs: supportedKemCipherSuite)
+  : ImplEdhocCrypto.aead_decrypt_st (Spec.get_aead_alg kcs) (aead_config_pre kcs)
+  = match (Spec.get_aead_alg kcs) with
+    | SpecAEAD.AES128_GCM -> ImplEdhocCrypto.aead_aes128_gcm_decrypt
+    | SpecAEAD.AES256_GCM -> ImplEdhocCrypto.aead_aes256_gcm_decrypt
+
+(*------------------ Hash*)
+inline_for_extraction
+let hash_pre (kcs: supportedKemCipherSuite)
+  : Type0
+  = match (Spec.get_hash_alg kcs) with
+    | SpecHash.SHA2_256 -> True
+
+let do_hash (kcs: supportedKemCipherSuite)
+  : ImplEdhocCrypto.do_hash_st (Spec.get_hash_alg kcs) (hash_pre kcs)
+  = match (Spec.get_hash_alg kcs) with
+    | SpecHash.SHA2_256 -> ImplEdhocCrypto.hash_sha2_256
+
+(*------------------ HKDF*)
+let hkdf_expand (kcs: supportedKemCipherSuite)
+  : ImplEdhocCrypto.hkdf_expand_st (Spec.get_hash_alg kcs)
+  = match (Spec.get_hash_alg kcs) with
+    | SpecHash.SHA2_256 -> ImplEdhocCrypto.hkdf_expand_sha2_256
+
+let hkdf_extract (kcs: supportedKemCipherSuite)
+  : ImplEdhocCrypto.hkdf_extract_st (Spec.get_hash_alg kcs)
+  = match (Spec.get_hash_alg kcs) with
+    | SpecHash.SHA2_256 -> ImplEdhocCrypto.hkdf_extract_sha2_256
+
+(*------------------ KEM*)
+// let kem_state = B.gcmalloc HyperStack.root 0ul 48ul
+let kem_state = ImplFrodoRand.state
+
+/// KEM key generation
+inline_for_extraction noextract
+type kem_keygen_st (a: supportedKemAlg)
+  = pk: alg_kem_pub_key_buff a
+  -> sk: alg_kem_priv_key_buff a
+  -> ST.Stack unit
+  (requires fun h0 ->
+    live h0 entropy_p /\ live h0 pk /\ live h0 sk
+    /\ B.all_disjoint [loc pk; loc sk; loc entropy_p; loc kem_state]
+  )
+  (ensures fun h0 _ h1 ->
+    modifies (loc kem_state |+| loc pk |+| loc sk |+| loc entropy_p) h0 h1
+    /\ (
+      let e0_v = B.deref h0 (entropy_p <: B.buffer (Ghost.erased HACLRandom.entropy)) in
+      let (pk_s, sk_s) = Spec.alg_kem_keygen a e0_v in
+
+      Seq.equal (as_seq h1 pk) pk_s
+      /\ Seq.equal (as_seq h1 sk) sk_s
+    )
+  )
+
+inline_for_extraction
+val kem_keygen_frodo640: kem_keygen_st Spec.Frodo640
+
+let kem_keygen (kcs: supportedKemCipherSuite)
+  = match (Spec.get_kem_alg kcs) with
+    | Spec.Frodo640 -> kem_keygen_frodo640
+
+/// KEM encapsulation
+inline_for_extraction noextract
+type kem_encaps_st (a: supportedKemAlg)
+  = pk: alg_kem_pub_key_buff a
+  -> ct: alg_kem_ciphertext_buff a
+  -> ss: alg_kem_shared_secret_buff a
+  -> ST.Stack unit
+  (requires fun h0 ->
+    live h0 entropy_p /\ live h0 pk /\ live h0 ct /\ live h0 ss
+    /\ B.all_disjoint [loc pk; loc entropy_p; loc kem_state; loc ct; loc ss]
+  )
+  (ensures fun h0 _ h1 ->
+    modifies (loc entropy_p |+| loc kem_state |+| loc ct |+| loc ss) h0 h1
+    /\ (
+      let e0_v = B.deref h0 (entropy_p <: B.buffer (Ghost.erased HACLRandom.entropy)) in
+      let pk_s = as_seq h0 pk in
+      let (ct_s, ss_s) = Spec.alg_kem_encaps a e0_v pk_s in
+
+      Seq.equal (as_seq h1 ct) ct_s
+      /\ Seq.equal (as_seq h1 ss) ss_s
+    )
+  )
+
+inline_for_extraction
+val kem_encaps_frodo640: kem_encaps_st Spec.Frodo640
+
+let kem_encaps (kcs: supportedKemCipherSuite)
+  = match (Spec.get_kem_alg kcs) with
+    | Spec.Frodo640 -> kem_encaps_frodo640
+
+/// KEM decapsulation
+inline_for_extraction noextract
+type kem_decaps_st (a: supportedKemAlg)
+  = sk: alg_kem_priv_key_buff a
+  -> ct: alg_kem_ciphertext_buff a
+  -> ss: alg_kem_shared_secret_buff a
+  -> ST.Stack unit
+  (requires fun h0 -> 
+    live h0 sk /\ live h0 ct /\ live h0 ss
+    /\ B.all_disjoint [loc sk; loc ct; loc ss]
+  )
+  (ensures fun h0 _ h1 ->
+    modifies1 ss h0 h1
+    /\ (
+      let ss_s = Spec.alg_kem_decaps a (as_seq h0 ct) (as_seq h0 sk) in
+      Seq.equal (as_seq h1 ss) ss_s
+    )
+  )
+
+inline_for_extraction
+val kem_decaps_frodo640: kem_decaps_st Spec.Frodo640
+
+let kem_decaps (kcs: supportedKemCipherSuite)
+  = match (Spec.get_kem_alg kcs) with
+    | Spec.Frodo640 -> kem_decaps_frodo640
