src/kemedhoc/Impl.KEMEDHOC.Types.fst
@@ -1,0 +1,126 @@
+module Impl.KEMEDHOC.Types
+
+open Lib.ByteBuffer
+open Lib.Buffer
+open Lib.IntTypes
+open Lib.ByteSequence
+open LowStar.BufferOps
+
+(*LowStar related modules*)
+module B = LowStar.Buffer
+module ST = FStar.HyperStack.ST
+module HS = FStar.HyperStack
+module S = FStar.Seq
+module Seq = Lib.Sequence
+
+(*Specification modules*)
+module SpecParser = Spec.KEMEDHOC.Parser
+
+open Spec.KEMEDHOC.CryptoPrimitives
+// module ImplEdhocCrypto = Impl.EDHOC.CryptoPrimitives
+module SpecEdhocCrypto = Spec.EDHOC.CryptoPrimitives
+
+/// The Low* type that represents an optional
+/// lbytes sequence
+noeq type lbufferOpt (len: size_t) = {
+  is_some: bool;
+  value: lbuffer uint8 len
+}
+
+/// Convert lbuffer_opt to `option lbytes`
+/// only for proofs
+let eval_lbuffer_opt (#len: size_t)
+  (h: HS.mem) (buff: lbufferOpt len)
+  : GTot (option (lbytes (size_v len)))
+  = if (buff.is_some)
+    then Some (as_seq h buff.value)
+    else None
+
+/// Plaintext buffers
+inline_for_extraction
+type plaintext1_buff = lbuffer uint8 (size SpecParser.plaintext1_size)
+inline_for_extraction
+type plaintext2_buff (kcs: supportedKemCipherSuite)
+  = lbuffer uint8 (size (SpecParser.plaintext2_size kcs))
+inline_for_extraction
+type plaintext3_buff (kcs: supportedKemCipherSuite)
+  = lbuffer uint8 (size (SpecParser.plaintext3_size kcs))
+
+/// Ciphertext buffers
+inline_for_extraction
+type c1_buff (kcs: supportedKemCipherSuite)
+  = lbuffer uint8 (size (SpecParser.c1_size kcs))
+inline_for_extraction
+type c2_buff (kcs: supportedKemCipherSuite)
+  = lbuffer uint8 (size (SpecParser.c2_size kcs))
+inline_for_extraction
+type c3_buff (kcs: supportedKemCipherSuite)
+  = lbuffer uint8 (size (SpecParser.c3_size kcs))
+
+
+(*Crypto Primitives buffer*)
+
+/// Alg-driven KEM buffers
+inline_for_extraction
+type alg_kem_pub_key_buff (a: kemAlg)
+  = lbuffer uint8 (size (alg_kem_public_key_size a))
+inline_for_extraction
+type alg_kem_priv_key_buff (a: kemAlg)
+  = lbuffer uint8 (size (alg_kem_priv_key_size a))
+inline_for_extraction
+type alg_kem_ciphertext_buff (a: kemAlg)
+  = lbuffer uint8 (size (alg_kem_ciphertext_size a))
+inline_for_extraction
+type alg_kem_shared_secret_buff (a: kemAlg)
+  = lbuffer uint8 (size (alg_kem_shared_secret_size a))
+
+/// Ciphersuite-driven KEM buffers
+inline_for_extraction
+type kem_pub_key_buff (kcs: kemCipherSuite)
+  = alg_kem_pub_key_buff (get_kem_alg kcs)
+inline_for_extraction
+type kem_priv_key_buff (kcs: kemCipherSuite)
+  = alg_kem_priv_key_buff (get_kem_alg kcs)
+inline_for_extraction
+type kem_ciphertext_buff (kcs: kemCipherSuite)
+  = alg_kem_ciphertext_buff (get_kem_alg kcs)
+inline_for_extraction
+type kem_shared_secret_size (kcs: kemCipherSuite)
+  = alg_kem_shared_secret_buff (get_kem_alg kcs)
+
+
+/// Hash out buffer
+// inline_for_extraction
+// type alg_hash_out_buff ()
+inline_for_extraction
+type hash_out_buff (kcs: kemCipherSuite)
+  = lbuffer uint8 (size (hash_size kcs))
+
+
+/// AEAD buffers
+inline_for_extraction
+type aead_tag_buff (kcs: kemCipherSuite)
+  = lbuffer uint8 (size (aead_tag_size kcs))
+inline_for_extraction
+type aead_iv_buff
+  = lbuffer uint8 (size aead_iv_size)
+inline_for_extraction
+type aead_key_buff (kcs: kemCipherSuite)
+  = lbuffer uint8 (size (aead_key_size kcs))
+inline_for_extraction
+type aead_valid_input_buff (kcs: kemCipherSuite)
+  = b:buffer_t MUT uint8{
+    length b <= SpecEdhocCrypto.alg_aead_max_input_size (get_aead_alg kcs)
+  }
+inline_for_extraction
+type aead_valid_ciphertext_buff (kcs: kemCipherSuite)
+  = b:buffer_t MUT uint8{
+    let tag_size = aead_tag_size kcs in
+    length b >= tag_size
+    /\ length b <= SpecEdhocCrypto.alg_aead_max_input_size (get_aead_alg kcs) + tag_size
+  }
+
+/// MAC23 buffer
+inline_for_extraction
+type mac23_buff (kcs: supportedKemCipherSuite)
+  = lbuffer uint8 (size (mac23_size kcs))
